tla-tree/ImmutableDiskTreeRefinement.dfy
@@ -1,0 +1,29 @@
+include "CrashableMap.dfy"
+include "ImmutableDiskTreeInterpretation.dfy"
+
+module ImmutableDiskTreeRefinement {
+import opened TreeTypes
+import opened ImmutableDiskTree
+import opened ImmutableDiskTreeInv
+import opened ImmutableDiskTreeHeight
+import opened ImmutableDiskTreeInterpretation
+import CrashableMap
+
+lemma InvImpliesRefinementInit(k:Constants, s:Variables)
+    requires Init(k, s)
+    requires TreeInv(k, s)
+    ensures CrashableMap.Init(Ik(k), I(k, s))
+{
+} 
+
+lemma InvImpliesRefinementNext(k:Constants, s:Variables, s':Variables)
+    requires Next(k, s, s')
+    requires TreeInv(k, s)
+    requires TreeInv(k, s')
+    ensures CrashableMap.WF(I(k, s))
+    ensures CrashableMap.WF(I(k, s'))
+    ensures CrashableMap.Next(Ik(k), I(k, s), I(k, s'))
+{
+}
+
+} // module ImmutableDiskTreeRefinement
